ver3_less_complex/Lemmas_Adversary.dfy
@@ -1,0 +1,34 @@
+include "Replica.dfy"
+include "Adversary.dfy"
+include "System.dfy"
+include "Type.dfy"
+include "Auxilarily.dfy"
+include "Axioms.dfy"
+include "common/proofs.dfy"
+
+module M_Lemmas_Adversary {
+
+    import opened M_Replica
+    import opened M_Adversary
+    import opened M_System
+    import opened M_SpecTypes
+    import opened M_AuxilarilyFunc
+    import opened M_Axiom
+    import opened M_ProofTactic
+
+    // lemma LemmaStableIDInAdversaryNext(
+    // ss : SystemState,
+    // inMsg : set<Msg>,
+    // ss' : SystemState,
+    // outMsg : set<Msg>
+    // )
+    // requires AdversaryNext(ss.adversary, inMsg, ss'.adversary, outMsg)
+    // ensures forall r | && r in ss.adversary.byz_nodes
+    //                    && r in ss.nodeStates.Keys
+    //                    && r in ss'.nodeStates.Keys
+    //                 ::
+    //                    ss.nodeStates[r].id == ss'.nodeStates[r].id
+    // {
+        
+    // }
+}
